Core/Automata2.v
@@ -22,9 +22,7 @@ Tactic Notation "spec" hyp(H) constr(a) constr(b) constr(c) :=
 Tactic Notation "spec" hyp(H) constr(a) constr(b) constr(c) constr(d) :=
   (generalize (H a b c d); clear H; intro H).
 
-
 (* A semantics of contracts with decidable deterministic transitions *)
-
 Section State.
 
 Definition value := nat.
@@ -51,13 +49,12 @@ Record cstate (T : Type) := CState {
 (* Global blockchain state *)
 Record bstate := BState {
       block_num : nat;
-      (* Anything else? *)
 }.
 
 End State.
 
 Section Protocol.
-
+  
 Section Transitions.
 
 (* State type *)
@@ -77,7 +74,7 @@ Record ctransition :=
       (* Unique tag of a transition in the protocol *)
       ttag : tag;
       
-      (* Funcion (bstate, state, msg) :-> (state', option msg') *)
+      (* Function (bstate, state, msg) :-> (state', option msg') *)
       tfun : trans_fun_type;
   }.
 
@@ -119,152 +116,36 @@ Fixpoint wf_sched (sch : schedule) :=
        all [pred s' | bnum <= block_num s'.1] sch' && wf_sched sch'
   else true.
 
-Record step :=
-  Step {
-      pre  : cstate S;
-      post : cstate S;
-      out  : option message
-  }.
-
-Definition trace := seq step.
-
-Definition apply_prot id bal s m bc : (S * option message) :=
-  let n  := seq.find (fun t => ttag t == method m) (transitions p) in
-  let tr := nth (idle S) (transitions p) n in
-  let f  := tfun tr in
-  f id bal s m bc.
-
-Definition step_prot pre bc m : step :=
+Definition step_state pre bc m : cstate S :=
   let: CState id bal s := pre in
-  let: (s', out) := apply_prot id bal s m bc in
+  let: n := seq.find (fun t => ttag t == method m) (transitions p) in
+  let: tr := nth (idle S) (transitions p) n in
+  let: (s', out) := (tfun tr) id bal s m bc in
   let: bal' := if out is Some m' then (bal + val m) - val m' else bal in
-  let: post := CState id bal' s' in
-  Step pre post out.
-
-(* Map a schedule into a trace *)
-Fixpoint execute (pre : cstate S) (sc: schedule) : trace :=
-  if sc is (bc, m) :: sc'
-  then let stp := step_prot pre bc m in
-       stp :: execute (post stp) sc'
-  else [::].
-
-
+  CState id bal' s'.
 
 Definition state0 := CState (acc p) (init_bal p) (init_state p).
 
-(* Execute from the initial contract state,
-   if schedule is empty, repeat the initial state *)
-Definition execute0 sc :=
-  if sc is _ :: _
-  then execute state0 sc
-  else [:: Step state0 state0 None].
-
-(****************************************************************)
-(* Safety property:
-For any state s in _any_ trace, starting from the initial one, 
-the unary property I holds (i.e., I s).
-*)
-(****************************************************************)
-(* Definition safe (I : cstate S -> Prop) : Prop :=
-  forall sc pre post out,
-    Step pre post out \In execute0 sc -> I pre /\ I post. *)
-
-Lemma bad_tag_step bc m s :
-  method m \notin (tags p) -> post (step_prot s bc m) = s.
-Proof.
-move=>M; rewrite /step_prot; case: s=>id bal s.
-rewrite [apply_prot _ _ _ _ _]surjective_pairing/=.
-rewrite /apply_prot.
-suff X : seq.find (fun t : ctransition S => ttag t == method m) (transitions p) =
-         size (transitions p).
-by rewrite !X !nth_default ?leqnn//.
-move: (find_size (fun t : ctransition S => ttag t == method m) (transitions p)).
-rewrite leq_eqVlt; case/orP; first by move/eqP.
-rewrite -has_find=>G. suff X: False by [].
-rewrite /tags in M; clear s bal id bc.
-elim: (transitions p) G M=>//t ts Hi/=.
-case/orP; last by move/Hi=>{Hi} Hi H; apply: Hi; rewrite inE in H; case/norP: H.
-by move/eqP=>->; rewrite inE eqxx.
-Qed.
-  
-(* A strong induction principle for proving safety *)
-(* Lemma safe_ind (I : cstate S -> Prop) :
-  I state0 ->
-  (forall pre bc m, 
-      (method m \in tags p) -> I pre -> I (post (step_prot pre bc m))) ->
-  safe I.
-Proof.
-move=>H1 H2; case=>[|[bc m] sc] pre pst out; first by case; case=>->->.
-case/In_cons=>[E|];[| rewrite -/execute].
-- have Z: pst = post (step_prot state0 bc m) by rewrite -E.
-  subst pst; split.
-  + suff Z: pre = state0 by subst pre.
-    move: E; rewrite /step_prot/=.
-    by rewrite [apply_prot _ _ _ _ _]surjective_pairing; case.
-  case M: (method m \in tags p); first by apply: H2.
-  by rewrite bad_tag_step// M.
-have Hp: I (post (step_prot state0 bc m)).
-- case M: (method m \in tags p); first by apply: H2.
-  by rewrite bad_tag_step// M.
-move: (post (step_prot state0 bc m)) Hp=>s Hi G; clear H1 bc m.
-elim: sc s Hi G=>//[[bc m] sc] Hi s Is.
-case/In_cons=>[E|];[|rewrite -/execute]; last first.
-- move/Hi=>H; apply: H.
-  case M: (method m \in tags p); first by apply: H2.
-  by rewrite bad_tag_step// M.
-suff Z: s = pre /\ pst = post (step_prot pre bc m).
-- case: Z=>??; subst pre pst; split=>//.
-  case M: (method m \in tags p); first by apply: H2.
-  by rewrite bad_tag_step// M.
-move: E; rewrite /step_prot/=; clear Is.
-case: s=>id bal s; rewrite [apply_prot _ _ _ _ _]surjective_pairing.
-by case=>->; rewrite {4}[apply_prot id bal s m bc]surjective_pairing.
-Qed.
-*)
 (*****************************************************)
 (*            Some modal connectives                 *)
 (*****************************************************)
+(* A temporal CTL semantics *)
 Definition pred := cstate S -> Prop.
-(* R needs to be implemented via the transitions *)
-Parameter R : cstate S -> cstate S -> Prop.
+Definition reachability : cstate S -> cstate S -> Prop := fun s1 s2 =>
+                                                          exists (bc : bstate) (m : message),
+                                                            step_state s1 bc m = s2.
 Definition path := nat -> cstate S.
-(* gpath is a sigma type *)
-(* Currently reachability is lazily defined as parameter R *)
+Definition first (p : path) : cstate S := p 0. 
 
-Definition path_predicate (p : path) := forall n, R (p n) (p (n + 1)).
+(* A good path is a path that begins with the initial state and satisfies the reachability relation *)
+Definition path_predicate (p : path) := (* p 0 = state0 /\ *) forall n, reachability (p n) (p (n + 1)).
 Definition gpath : Type := {p : path & path_predicate p }.
-
-(* Parameter gpath : {p : path & path_predicate p }. 
-
-
-Definition projT1 (x:sigT path_predicate) : path := match x with
-                                      | existT a _ => a
-                                                    end.
-
-Definition good_path := projT1 gpath.
-Check good_path. *)
-(* 
-Definition projT1_sig (e:sig path_predicate) := match e with
-                                    | exist a b => a
-                                                end. *)
-
 Definition gpath_proj1 : gpath -> (nat -> cstate S) := fun gp =>  match gp with | existT a _ => a end.
-Definition gpath_proj1' : (sigT path_predicate) -> (nat -> cstate S) := fun gp => match gp with |existT a _ => a end.
-Lemma blah : gpath_proj1 = gpath_proj1'.
-  reflexivity.
-Locate sigT.
-
 Coercion gpath_proj1 : gpath >-> Funclass.
 
-Definition first (p : gpath) : cstate S := p 0.
-
+(* State satisfaction *)
 Definition forces (s : cstate S) (p : pred) : Prop :=
   p s.
-
-Parameter Top : pred.
-Parameter Bottom : pred.
-
-(* Notation *)
 Notation "w '|=' P" := (forces w P) (at level 80, no associativity).
 
 (* Stuff in Prop *)
@@ -275,6 +156,8 @@ Definition equiv P Q : Prop :=
   entails P Q /\ entails Q P.
 
 (* Stuff in pred *)
+Parameter Top : pred.
+Parameter Bottom : pred.
 Definition Neg P : pred := fun w =>
                              ~(w |= P).
 Definition Conj P Q : pred := fun w =>
@@ -285,16 +168,11 @@ Definition Impl P Q : pred := fun w =>
                                 ~(w |= P) \/ (w |= Q).
 
 Delimit Scope temporal_logic with temporal_logic.
-Local Open Scope temporal_logic.
+Open Scope temporal_logic.
 
 Notation "P <=> Q" := (equiv P Q) (at level 35, no associativity).
-
-(* Metalogic semantics *)
-(* Definition Top : pred := fun w =>
-                           ~ (w |= Bottom). *)                        
-
 Notation "~~ P" := (Neg P) : temporal_logic.
-Notation "P & Q" := (Conj P Q) (at level 35, no associativity) : temporal_logic.
+Notation "P & Q" := (Conj P Q) (at level 65, left associativity) : temporal_logic.
 Notation "P || Q" := (Disj P Q) : temporal_logic.
 Notation "P --> Q" := (Impl P Q) (at level 35, no associativity) : temporal_logic.
 
@@ -336,6 +214,8 @@ Definition AllWait P Q : pred :=
 Definition ExistsWait P Q : pred :=
   ExistsRelease P (P || Q).
 
+Close Scope temporal_logic.
+
 (* Given the sigma-type gpath, we can safely say this
 because gpath will handle the proof of reachability *)
 Definition reachable (st st' : cstate S) :=
@@ -343,47 +223,24 @@ Definition reachable (st st' : cstate S) :=
   exists (n m : nat),
     p n = st /\ p m = st.
 
-(* 
-Definition reachable' (st st' : cstate S) sc :=
-  st' = post (last (Step st st None) (execute st sc)).
-
-Definition reachable (st st' : cstate S) :=
-  exists sc, reachable' st st' sc.
- *)
-
-(* q holds since p , as long as schedule bits satisfy r. 
-Definition since_as_long
-           (p : cstate S -> Prop)
-           (q : cstate S -> cstate S -> Prop)
-           (r : bstate * message -> Prop) :=
-  forall sc st st',
-    p st ->
-    (forall b, b \In sc -> r b) ->
-    reachable' st st' sc ->
-    q st st'. *)
-
 (* A stronger safety property *)
 (* The former safety property said that all states in a viable execution path
 hold a certain property *)
 (* If we assume that "path" already comes with a viability *)
-Definition safe (P : pred) (p : path) :=
+Definition safe (P : pred) (p : gpath) :=
   forall n : nat, P (p n).
 
 Lemma safe_ind :
-  forall (P : pred) (p : path),
+  forall (P : pred) (p : gpath),
   P (p 0) ->
   (forall n : nat, P (p n) -> P (p (n.+1))) ->
                   forall n : nat, P (p n).
 Proof.
   intros P path.
-  intros H_0 HI m.
+  intros H_0 HI m. 
   elim m.
   exact H_0.
-  Search (_.+ _).
-  Locate ptrA.
   apply HI.
 Qed. 
-  (* This allows us to directly borrow from the inductive structure
-of natural numbers *)
 
 End Semantics.
