Core/.#Automata2.v
@@ -1,1 +1,0 @@
-Elaine@Elaines-MacBook-Pro-5.local.93092
